Demo.v
@@ -281,7 +281,7 @@ Compute (expr_eval_n 10 Σ [] [| {plus_syn} 0 |]).
 
 Definition fun_app := [| (\x : Nat -> \y : Nat -> y + x) Z |].
 
-Compute (expr_eval_n 10 [] [] fun_app).
+Compute (expr_eval_n 10 Σ [] fun_app).
 
 Example fun_app_from_val :
   exists v, (expr_eval_n 10 Σ' [] (indexify [] fun_app)) = Ok v /\
