WcbvEval1.v
@@ -1,0 +1,377 @@
+(* Distributed under the terms of the MIT license.   *)
+
+From Coq Require Import Bool String List Program BinPos Compare_dec Omega.
+From Template Require Import config utils Ast univ Induction LiftSubst UnivSubst Typing.
+From Template Require Import AstUtils.
+Require Import Facts CustomTactics.
+Require Import String.
+Local Open Scope string_scope.
+Set Asymmetric Patterns.
+
+Existing Instance default_checker_flags.
+
+(** * Weak (head) call-by-value evaluation strategy.
+
+  The [wcbveval] inductive relation specifies weak cbv evaluation.  It
+  is shown to be a subrelation of the 1-step reduction relation from
+  which conversion is defined. Hence two terms that reduce to the same
+  wcbv head normal form are convertible.
+
+  This reduction strategy is supposed to mimick at the Coq level the
+  reduction strategy of ML programming languages. It is used to state
+  the extraction conjecture that can be applied to Coq terms to produce
+  (untyped) terms where all proofs are erased to a dummy value. *)
+
+(** ** Big step version of weak cbv beta-zeta-iota-fix-delta reduction.
+
+  TODO: CoFixpoints *)
+
+(* We define a notion of atom for terms that reduce to themselves, when
+   they are not applied.
+
+   We do not include [Rel] which is handled specially, [Var] and [Meta]
+   which are out of scope. We assume no axioms either, that is constants
+   with no bodies.
+
+*)
+
+Definition atom t :=
+  match t with
+  | tSort _
+  | tInd _ _
+  | tConstruct _ _ _
+  | tFix _ _
+  | tCoFix _ _ => true
+  | _ => false
+  end.
+
+Definition mkApps' (t : term) (ts : list term):=
+  match ts with
+  | [] => t
+  | _ => tApp t ts
+  end.
+
+
+Fixpoint flat_apps (t  : term) : bool :=
+  match t  with
+  | tRel x => true
+  | tVar x => true
+  | tMeta x => true
+  | tEvar x x0 => true
+  | tSort x => true
+  | tCast t1 _ t2 => flat_apps t1 && flat_apps t2
+  | tProd _ t1 t2 => flat_apps t1 && flat_apps t2
+  | tLambda _ t1 t2 => flat_apps t1 && flat_apps t2
+  | tLetIn nm t1 t2 t3 => flat_apps t1 && flat_apps t2 && flat_apps t3
+  | tApp t ts => negb (isApp t) && forallb flat_apps ts
+  | tConst _ _ => true
+  | tInd _ _ => true
+  | tConstruct _ _ _ => true
+  | tCase _ t1 t2 bs => flat_apps t1 && flat_apps t2 && forallb (test_snd (flat_apps)) bs
+  | tProj _ t => flat_apps t
+  | tFix mfx _ => forallb (test_def flat_apps) mfx
+  | tCoFix mfx _ => forallb (test_def flat_apps) mfx
+  end.
+
+
+Lemma lift_flat_apps t n m :
+  flat_apps t -> flat_apps (lift n m t ).
+Proof.
+Admitted.
+
+Hint Resolve <- negb_true_iff : facts.
+Hint Resolve -> negb_true_iff : facts.
+
+Lemma flat_apps_no_apps t t1 ts :
+  flat_apps t -> t = tApp t1 ts -> isApp t1 = false /\ forallb flat_apps ts = true.
+Proof.
+  intros Happ Heq. subst. simpl in *. inv_andb Happ;split;eauto with facts.
+Qed.
+
+Lemma subst_flattens t u n:
+  flat_apps u ->
+  flat_apps (t{n:=u}).
+Proof.
+  revert u n.
+  induction t using Induction.term_forall_list_ind;simpl;intros u1 n1 Hu1;eauto.
+  + destruct (n1 ?= n);auto. now apply lift_flat_apps.
+  + split_andb. now apply IHt1. now apply IHt2.
+  + split_andb. now apply IHt1. now apply IHt2.
+  + split_andb. now apply IHt1. now apply IHt2.
+  + repeat split_andb. now apply IHt1. now apply IHt2.  now apply IHt3.
+  + destruct l.
+    * simpl. easy.
+    * inversion H as [a | a b Ht0 Hfa];subst;clear H.
+      destruct (isApp (t {n1 := u1})) eqn:Ht.
+      ** destruct (t {n1 := u1}) eqn:Htsubst;auto;inversion Ht.
+         assert (flat_apps (t {n1 := u1})) by easy.
+         simpl in *.
+         unfold is_true.
+         assert (Happ : isApp t1 = false /\ forallb flat_apps l0 = true).
+         { eapply flat_apps_no_apps;eauto. }
+         destruct Happ. split_andb;eauto with facts.
+         rewrite forallb_app. split_andb;eauto with facts.
+         simpl. split_andb. apply Ht0;easy.
+         rewrite forallb_map.
+         eapply Forall_forallb;eauto.
+      ** rewrite mkApps_tApp. simpl.
+         split_andb;eauto with facts.
+         split_andb. now apply Ht0.
+         rewrite forallb_map.
+         eapply Forall_forallb;eauto. intros H;tryfalse.
+         intros H;tryfalse.
+  +
+Admitted.
+
+
+Section Wcbv.
+  Context (Σ : global_declarations) (Γ : context).
+  (* The local context is fixed: we are only doing weak reductions *)
+
+  Inductive eval : term -> term -> Prop :=
+  (** Reductions *)
+  (** Beta *)
+  | eval_beta t a l res :
+      eval_apps t (a :: l) res ->
+      eval (tApp t (a :: l)) res
+
+  (** Let *)
+  | eval_zeta na b0 b0' t b1 res :
+      eval b0 b0' ->
+      eval (subst0 b0' b1) res ->
+      eval (tLetIn na b0 t b1) res
+
+  (** Local variables: defined or undefined *)
+  | eval_rel_def i (isdecl : i < List.length Γ) body res :
+      (safe_nth Γ (exist _ i isdecl)).(decl_body) = Some body ->
+      eval (lift0 (S i) body) res ->
+      eval (tRel i) res
+
+  | eval_rel_undef i (isdecl : i < List.length Γ) :
+      (safe_nth Γ (exist _ i isdecl)).(decl_body) = None ->
+      eval (tRel i) (tRel i)
+
+  (** Case *)
+  | eval_iota ind pars discr c u args p brs res :
+      eval discr (mkApps (tConstruct ind c u) args) ->
+      eval (iota_red pars c args brs) res ->
+      eval (tCase (ind, pars) p discr brs) res
+
+  (** Constant unfolding *)
+  | eval_delta c decl body (isdecl : declared_constant Σ c decl) u res :
+      decl.(cst_body) = Some body ->
+      eval (subst_instance_constr u body) res ->
+      eval (tConst c u) res
+
+  (** Proj *)
+  | eval_proj i pars arg discr args k u res :
+      eval discr (mkApps (tConstruct i k u) args) ->
+      eval (List.nth (pars + arg) args tDummy) res ->
+      eval (tProj (i, pars, arg) discr) res
+
+  (* TODO CoFix *)
+  | eval_abs na M N : eval (tLambda na M N) (tLambda na M N)
+
+  | eval_prod na b t : eval (tProd na b t) (tProd na b t)
+
+  | eval_atom t : atom t = true -> eval t t
+
+  | eval_evar ev l : eval (tEvar ev l) (tEvar ev l) (* Lets say it is a value for now *)
+
+  | eval_cast M1 k M2 N1 : eval M1 N1 -> eval (tCast M1 k M2) N1
+  with
+  eval_apps : term -> list term -> term -> Prop :=
+  | eval_app_lam f na t b a a' l res :
+      eval f (tLambda na t b) ->
+      eval a a' ->
+      eval_apps (subst0 a' b) l res ->
+      eval_apps f (a :: l) res
+  | eval_app_empty t res :
+      eval t res ->
+      eval_apps t [] res
+  | eval_app_constr a f i k u l l' :
+      eval f (tConstruct i k u) ->
+      All2 eval (a :: l) l' ->
+      eval_apps f (a :: l) (tApp (tConstruct i k u) l')
+  | eval_app_ind a t i u l l' :
+      eval t (tInd i u) ->
+      All2 eval (a :: l) l' ->
+      eval_apps t (a :: l) (tApp (tInd i u) l')
+
+    (** Fix unfolding, with guard *)
+  | eval_fix mfix idx args args' narg fn res :
+      unfold_fix mfix idx = Some (narg, fn) ->
+      All2 eval args args' -> (* FIXME should we reduce the args after the recursive arg here? *)
+      is_constructor narg args' = true ->
+      eval_apps fn args' res ->
+      eval_apps (tFix mfix idx) args res.
+
+  (* | eval_fix mfix idx args args' a narg fn res l : *)
+  (*     unfold_fix mfix idx = Some (narg, fn) -> *)
+  (*     All2 eval args args' -> (* FIXME should we reduce the args after the recursive arg here? *) *)
+  (*     is_constructor 0 [a] = true -> *)
+  (*     eval_apps fn args' res -> *)
+  (*     eval_apps (tFix (mkdef nm dty dbody 0) idx) (a :: l) res. *)
+
+
+  (** The right induction principle for the nested [Forall] cases: *)
+
+  Lemma eval_evals_ind :
+    forall P : term -> term -> Prop,
+      (forall (f : term) (na : name) (t b a a' : term) (l : list term) (res : term),
+          eval f (tLambda na t b) ->
+          P f (tLambda na t b) ->
+          eval a a' -> P a a' ->
+          eval (mkApps' (b {0 := a'}) l) res -> P (mkApps (b {0 := a'}) l) res -> P (tApp f (a :: l)) res) ->
+
+      (forall (na : name) (b0 b0' t b1 res : term),
+          eval b0 b0' -> P b0 b0' -> eval (b1 {0 := b0'}) res -> P (b1 {0 := b0'}) res -> P (tLetIn na b0 t b1) res) ->
+
+      (forall (i : nat) (isdecl : i < #|Γ|) (body res : term),
+          decl_body (safe_nth Γ (exist (fun n : nat => n < #|Γ|) i isdecl)) = Some body ->
+          eval ((lift0 (S i)) body) res -> P ((lift0 (S i)) body) res -> P (tRel i) res) ->
+
+      (forall (i : nat) (isdecl : i < #|Γ|),
+          decl_body (safe_nth Γ (exist (fun n : nat => n < #|Γ|) i isdecl)) = None -> P (tRel i) (tRel i)) ->
+
+      (forall (ind : inductive) (pars : nat) (discr : term) (c : nat) (u : universe_instance)
+              (args : list term) (p : term) (brs : list (nat * term)) (res : term),
+          eval discr (mkApps (tConstruct ind c u) args) ->
+          P discr (mkApps (tConstruct ind c u) args) ->
+          eval (iota_red pars c args brs) res ->
+          P (iota_red pars c args brs) res -> P (tCase (ind, pars) p discr brs) res) ->
+
+      (forall (mfix : mfixpoint term) (idx : nat) (args args' : list term) (narg : nat) (fn res : term),
+          unfold_fix mfix idx = Some (narg, fn) ->
+          All2 eval args args' ->
+          All2 P args args' ->
+          is_constructor narg args' = true ->
+          eval (mkApps fn args') res -> P (mkApps fn args') res -> P (tApp (tFix mfix idx) args) res) ->
+
+      (forall (c : ident) (decl : constant_body) (body : term),
+          declared_constant Σ c decl ->
+          forall (u : universe_instance) (res : term),
+            cst_body decl = Some body ->
+            eval (subst_instance_constr u body) res -> P (subst_instance_constr u body) res -> P (tConst c u) res) ->
+
+      (forall (i : inductive) (pars arg : nat) (discr : term) (args : list term) (k : nat)
+              (u : universe_instance) (res : term),
+          eval discr (mkApps (tConstruct i k u) args) ->
+          P discr (mkApps (tConstruct i k u) args) ->
+          eval (nth (pars + arg) args tDummy) res ->
+          P (nth (pars + arg) args tDummy) res -> P (tProj (i, pars, arg) discr) res) ->
+
+      (forall (na : name) (M N : term), P (tLambda na M N) (tLambda na M N)) ->
+
+      (forall (na : name) (M N : term), P (tProd na M N) (tProd na M N)) ->
+
+      (forall (f8 : term) (i : inductive) (u : universe_instance) (l l' : list term),
+          l <> nil -> eval f8 (tInd i u) ->
+          P f8 (tInd i u) -> All2 eval l l' -> All2 P l l' -> P (tApp f8 l) (tApp (tInd i u) l')) ->
+
+      (forall (f8 : term) (i : inductive) (k : nat) (u : universe_instance) (l l' : list term),
+          l <> nil -> eval f8 (tConstruct i k u) ->
+          P f8 (tConstruct i k u) -> All2 eval l l' -> All2 P l l' -> P (tApp f8 l) (tApp (tConstruct i k u) l')) ->
+
+      (forall (t : term), atom t = true -> P t t) ->
+
+      (forall (ev : nat) (l : list term), P (tEvar ev l) (tEvar ev l)) ->
+
+      (forall (M1 : term) (k : cast_kind) (M2 N1 : term), eval M1 N1 -> P M1 N1 -> P (tCast M1 k M2) N1) ->
+
+      forall t t0 : term, eval t t0 -> P t t0.
+  Proof.
+    intros P Hbeta Hlet Hreldef Hrelvar Hcase Hfix Hconst Hproj Hlam Hprod Hindapp Hcstrapp Hatom Hevar Hcast.
+    fix eval_evals_ind 3. destruct 1;
+             try match goal with [ H : _ |- _ ] =>
+                             match type of H with
+                             | forall t t0, eval t t0 -> _ => fail 1
+                             | context [ atom _ ] => fail 1
+                             | _ => eapply H
+                             end end; eauto.
+    (* clear H1. *)
+  (*   (* clear H2. *) *)
+  (*   revert args args' H0. fix aux 3. destruct 1.  constructor; auto. *)
+  (*   constructor. now apply eval_evals_ind. now apply aux. *)
+  (*   revert l l' H H1. fix aux 4. destruct 2. contradiction. constructor. *)
+  (*   now apply eval_evals_ind. *)
+  (*   destruct l. inv H1; constructor. *)
+  (*   now apply aux. *)
+  (*   revert l l' H H1. fix aux 4. destruct 2. contradiction. constructor. *)
+  (*   now apply eval_evals_ind. destruct l. inv H1; constructor. now apply aux. *)
+    (* Defined. *)
+  Admitted.
+
+  (** Characterization of values for this reduction relation:
+      Basically atoms (constructors, inductives, products (FIXME sorts missing))
+      and de Bruijn variables and lambda abstractions. Closed values disallow
+      de Bruijn variables. *)
+
+  Inductive value : term -> Prop :=
+  | value_tRel i : value (tRel i)
+  | value_tEvar ev l : value (tEvar ev l)
+  | value_tLam na t b : value (tLambda na t b)
+  | value_tProd na t u : value (tProd na t u)
+  | value_tInd i k l : All value l -> value (mkApps (tInd i k) l)
+  | value_tConstruct i k u l : All value l -> value (mkApps (tConstruct i k u) l)
+  | value_atom t : atom t = true -> value t.
+
+  Lemma value_values_ind : forall P : term -> Prop,
+       (forall i : nat, P (tRel i)) ->
+       (forall (ev : nat) (l : list term), P (tEvar ev l)) ->
+       (forall (na : name) (t b : term), P (tLambda na t b)) ->
+       (forall (na : name) (t u : term), P (tProd na t u)) ->
+       (forall (i : inductive) (k : universe_instance) l,
+           All value l ->
+           All P l -> P (mkApps (tInd i k) l)) ->
+       (forall (i : inductive) (k : nat) (u : universe_instance) (l : list term),
+        All value l -> All P l -> P (mkApps (tConstruct i k u) l)) ->
+       (forall t, atom t = true -> P t) ->
+       forall t : term, value t -> P t.
+  Proof.
+    intros P ???????.
+    fix value_values_ind 2. destruct 1. 1-4:clear value_values_ind; auto.
+    apply H3. auto.
+    revert l H6. fix aux 2. destruct 1. constructor; auto.
+    constructor. now apply value_values_ind. now apply aux.
+    apply H4. apply H6.
+    revert l H6. fix aux 2. destruct 1. constructor; auto.
+    constructor. now apply value_values_ind. now apply aux.
+    now apply H5.
+  Defined.
+
+  (** The codomain of evaluation is only values:
+      It means no redex can remain at the head of an evaluated term. *)
+
+  Lemma eval_to_value e e' : eval e e' -> value e'.
+  Proof.
+    induction 1 using eval_evals_ind; simpl; auto using value.
+    pose (value_tInd i u l'). apply All2_right in H2.
+    rewrite mkApps_tApp in v; auto. simpl; auto. eauto using All2_non_nil.
+    pose proof (value_tConstruct i k u l'). forward H3.
+    apply (All2_right H2).
+    rewrite mkApps_tApp in H3; auto. simpl; auto. eauto using All2_non_nil.
+  Qed.
+
+  (** Evaluation preserves closedness: *)
+  Lemma eval_closed : forall n t u, closedn n t = true -> eval t u -> closedn n u = true.
+  Proof.
+    induction 2 using eval_evals_ind; simpl in *; eauto 2. eapply IHeval3.
+    admit.
+    eapply IHeval2.
+  Admitted. (* FIXME complete *)
+
+End Wcbv.
+
+(** Well-typed closed programs can't go wrong: they always evaluate to a value. *)
+
+Conjecture closed_typed_wcbeval : forall (Σ : global_context) t T,
+    Σ ;;; [] |- t : T -> { u & eval (fst Σ) [] t u }.
+
+(** Evaluation is a subrelation of reduction: *)
+
+Lemma wcbeval_red : forall (Σ : global_declarations) Γ t u,
+    eval Σ Γ t u -> red Σ Γ t u.
+Proof.
+  induction 1; try constructor; eauto.
+Admitted. (** TODO: Congruence lemmas of red for all constructions (as done in Coq in Coq) *)
